Interaction_Trees.thy
@@ -658,11 +658,9 @@ definition retvals :: "('e, 's) itree \<Rightarrow> 's set" ("\<^bold>R") where
 lemma retvals_traceI: "P \<midarrow>es\<leadsto> Ret x \<Longrightarrow> x \<in> \<^bold>R(P)"
   by (auto simp add: retvals_def)
 
-abbreviation "nonterminates P \<equiv> (\<^bold>R(P) = {})"
+abbreviation "nonterminating P \<equiv> (\<^bold>R(P) = {})"
 
-abbreviation "terminates P \<equiv> (\<^bold>R(P) \<noteq> {})"
-
-lemma nonterminates_iff: "nonterminates P \<longleftrightarrow> (\<forall> es x. \<not> P \<midarrow>es\<leadsto> \<checkmark> x)"
+lemma nonterminates_iff: "nonterminating P \<longleftrightarrow> (\<forall> es x. \<not> P \<midarrow>es\<leadsto> \<checkmark> x)"
   by (auto simp add: retvals_def)
 
 lemma retvals_Ret [simp]: "\<^bold>R(Ret x) = {x}"
@@ -682,6 +680,8 @@ lemma retvals_bind [simp]: "\<^bold>R(P \<bind> Q) = \<Union> {\<^bold>R (Q x)| 
   apply (metis mem_Collect_eq trace_to_Nil)
   apply (meson trace_to_bind)
   done
+
+subsection \<open> Termination \<close>
 
 subsection \<open> Event Alphabet \<close>
 
